ShadowingFree.v
@@ -1,0 +1,74 @@
+Require Import CSet Le.
+
+Require Import Plus Util AllInRel Map.
+Require Import Val Var Env EnvTy IL Annotation Liveness Restrict Bisim MoreExp SetOperations.
+Require Import DecSolve RenamedApart LabelsDefined.
+
+Set Implicit Arguments.
+
+(* shadowing free *)
+Inductive shadowing_free : set var -> stmt -> Prop :=
+  | shadowing_freeExp x e s D
+    : x ∉ D
+      -> Exp.freeVars e ⊆ D
+      -> shadowing_free {x; D} s
+      -> shadowing_free D (stmtLet x e s)
+  | shadowing_freeIf D e s t
+    : Exp.freeVars e ⊆ D
+    -> shadowing_free D s
+    -> shadowing_free D t
+    -> shadowing_free D (stmtIf e s t)
+  | shadowing_freeRet D e
+    : Exp.freeVars e ⊆ D
+    -> shadowing_free D (stmtReturn e)
+  | shadowing_freeGoto D f Y
+    : list_union (List.map Exp.freeVars Y) ⊆ D
+    -> shadowing_free D (stmtApp f Y)
+  | shadowing_freeExtern x f Y s D
+    : x ∉ D
+      -> list_union (List.map Exp.freeVars Y) ⊆ D
+      -> shadowing_free {x; D} s
+      -> shadowing_free D (stmtExtern x f Y s)
+  | shadowing_freeLet D s t Z
+    : of_list Z ∩ D [=] ∅
+    -> shadowing_free (of_list Z ∪ D) s
+    -> shadowing_free D t
+    -> shadowing_free D (stmtFun Z s t).
+
+Lemma shadowing_free_ext s D D'
+  : D' [=] D
+  -> shadowing_free D s
+  -> shadowing_free D' s.
+Proof.
+  intros EQ SF. general induction SF; simpl; econstructor; try rewrite EQ; eauto.
+  - eapply IHSF; eauto.
+    rewrite EQ; reflexivity.
+  - eapply IHSF; eauto. rewrite EQ; reflexivity.
+  - eapply IHSF1; eauto. rewrite EQ. reflexivity.
+Qed.
+
+Instance shadowing_free_morphism
+: Proper (Equal ==> eq ==> iff) shadowing_free.
+Proof.
+  unfold Proper, respectful; intros; subst.
+  split; eapply shadowing_free_ext; eauto. symmetry; eauto.
+Qed.
+
+Lemma renamedApart_shadowing_free s an
+  : renamedApart s an -> shadowing_free (fst (getAnn an)) s.
+Proof.
+  intros. general induction H; simpl; eauto using shadowing_free.
+  - econstructor; eauto. rewrite H2 in IHrenamedApart. eauto.
+  - rewrite H4 in IHrenamedApart1. rewrite H5 in IHrenamedApart2.
+    econstructor; eauto.
+  - econstructor; eauto. rewrite H2 in IHrenamedApart; eauto.
+  - rewrite H3 in IHrenamedApart1. rewrite H5 in IHrenamedApart2.
+    econstructor; eauto.
+Qed.
+
+
+(*
+*** Local Variables: ***
+*** coq-load-path: (("." "Lvc")) ***
+*** End: ***
+*)
